matching-logic/nix/deps.nix
@@ -30,4 +30,29 @@ let
         installFlags = [ "COQLIB=$(out)/lib/coq/${coq.coq-version}/" ];
       } ) { } ;
 
-in { inherit stdpp; coq = ncoq; }
+   equations = ncoqPackages.callPackage
+    ( { coq, stdenv, fetchFromGithub }:
+      stdenv.mkDerivation {
+        name = "coq${coq.coq-version}-stdpp";
+
+        src = fetchGit {
+          url = "https://github.com/mattam82/Coq-Equations.git";
+          ref = "8.13";
+          rev = "68c6907e49f4e1d69721ef4270ef8f3a302ae840";
+        };
+
+        postPatch = ''
+          patchShebangs --build configure.sh
+        '';
+        configurePhase = "./configure.sh";
+
+        buildInputs = with coq.ocamlPackages; [ ocaml camlp5 zarith findlib ];
+        propagatedBuildInputs = [ coq ];
+        enableParallelBuilding = true;
+
+        installFlags = [ "COQLIB=$(out)/lib/coq/${coq.coq-version}/" ];
+      } ) { } ;
+
+
+
+in { inherit stdpp; coq = ncoq; inherit equations; }
