prover/nix/deps.nix
@@ -14,36 +14,13 @@ let
 
   mllib = import ../../matching-logic/default.nix { inherit coqVersion;  };
 
-   equations = ncoqPackages.callPackage
-    ( { coq, stdenv, fetchFromGithub }:
-      stdenv.mkDerivation {
-        name = "coq${coq.coq-version}-stdpp";
-
-        src = fetchGit {
-          url = "https://github.com/mattam82/Coq-Equations.git";
-          ref = "8.13";
-          rev = "a7f1a02745092f4ddce4f91d0a5d69fb85376c34";
-        };
-
-        postPatch = ''
-          patchShebangs --build configure.sh
-        '';
-        configurePhase = "./configure.sh";
-
-        buildInputs = with coq.ocamlPackages; [ ocaml camlp5 zarith findlib ];
-        propagatedBuildInputs = [ coq ];
-        enableParallelBuilding = true;
-
-        installFlags = [ "COQLIB=$(out)/lib/coq/${coq.coq-version}/" ];
-      } ) { } ;
-
     metamath = pkgs.metamath;
     ocaml = coq.ocamlPackages.ocaml;
     camlp5 = coq.ocamlPackages.camlp5;
     findlib = ncoq.ocamlPackages.findlib;
     zarith = ncoq.ocamlPackages.zarith;
 
-in { coq = ncoq; inherit equations; inherit metamath; inherit mllib;
+in { coq = ncoq; inherit metamath; inherit mllib;
   inherit ocaml; inherit camlp5;
   inherit findlib; inherit zarith;
 }
